First pass at unifying var equal definitions and lemmas

CrIdentifiers.v
@@ -57,22 +57,25 @@ Proof.
     congruence.
 Defined.
 
+Instance CrVarLike_Ctrl : CrVarLike Ctrl.
+Proof.
+  refine {| make_item := fun uid => CtrlCtr uid;
+            get_key := fun s => match s with CtrlCtr uid => uid end;
+            inverses := _;
+            inj := _ |}.
+  - (* inverses : forall x, make_item (get_key x) = x *)
+    intros [uid]. simpl. reflexivity.
+  - (* inj : injective_contravariant get_key *)
+    intros x y Hxy Heq.
+    destruct x as [uid1], y as [uid2]; simpl in Heq.
+    rewrite Heq in Hxy.
+    congruence.
+Defined.
+
 (* Equality check functions for the identifiers above *)
 Definition parser_state_equal (p1 p2 : ParserState) :=
     match p1, p2 with
             | ParserStateCtr xid, ParserStateCtr yid => Pos.eqb xid yid
-    end.
-
-(* Do the same thing as parser_state_equal for Header *)
-Definition header_equal (h1 h2 : Header) :=
-    match h1, h2 with
-    | HeaderCtr xid, HeaderCtr yid => Pos.eqb xid yid
-    end.
-
-(* Do the same thing as parser_state_equal for State *)
-Definition state_equal (sv1 sv2 : State) :=
-    match sv1, sv2 with
-    | StateCtr xid, StateCtr yid => Pos.eqb xid yid
     end.
 
 (* Do the same thing as parser_state_equal for ModuleName *)
@@ -93,112 +96,50 @@ Definition connection_name_equal (c1 c2 : ConnectionName) :=
             | ConnectionNameCtr xid, ConnectionNameCtr yid => Pos.eqb xid yid
     end.
 
-(* Do the same thing as parser_state_equal for Ctrl *)
-Definition ctrl_equal (cc1 cc2 : Ctrl) :=
-    match cc1, cc2 with
-    | CtrlCtr xid, CtrlCtr yid => Pos.eqb xid yid
+Section CrVarLikeEqual.
+  Context {A : Type} `{CrVarLike A}.
+
+  Definition varlike_equal (v1 v2 : A) :=
+    Pos.eqb (get_key v1) (get_key v2).
+
+  Lemma varlike_equal_lemma :
+    forall v1 v2,
+    varlike_equal v1 v2 = true ->
+    v2 = v1.
+  Proof.
+    intros.
+    unfold varlike_equal in H0.
+    apply Pos.eqb_eq in H0.
+    rewrite <- inverses.
+    rewrite H0.
+    rewrite inverses.
+    reflexivity.
+  Qed.
+
+  Fixpoint varlike_list_equal (v1 v2 : list A) :=
+    match v1, v2 with
+    | nil, nil => true
+    | v::y, v'::y' => andb (varlike_equal v v') (varlike_list_equal y y')
+    | _, _ => false
     end.
 
-Lemma header_equal_lemma :
-  forall h1 h2,
-  header_equal h1 h2 = true ->
-  h1 = h2.
-Proof.
-  intros h1 h2 H.
-  destruct h1, h2; simpl in H; try congruence.
-  apply Pos.eqb_eq in H. subst. reflexivity.
-Qed.
-
-Fixpoint hdr_list_equal (h1 : list Header) (h2 : list Header) :=
-  match h1, h2 with
-  | nil, nil => true
-  | h::y, h'::y' => andb (header_equal h h') (hdr_list_equal y y')
-  | _, _ => false
-  end.
-       
-Lemma hdr_list_equal_lemma:
-  forall h1 h2,
-  hdr_list_equal h1 h2 = true ->
-  h1 = h2.
-Proof.
-  intros h1.
-  induction h1 as [|h1' h1''].
-  - destruct h2; simpl; congruence.
-  - destruct h2 as [|h2' h2''].
-    + simpl. congruence.
-    + intros H. simpl in H.
-      rewrite andb_true_iff in H. destruct H as [H1 H2].
-      apply header_equal_lemma in H1. subst. f_equal.
-      apply IHh1''.
-      assumption.
-Qed.
-
-Lemma state_equal_lemma :
-  forall s1 s2,
-  state_equal s1 s2 = true ->
-  s1 = s2.
-Proof.
-  intros s1 s2 H.
-  destruct s1, s2; simpl in H; try congruence.
-  apply Pos.eqb_eq in H. subst. reflexivity.
-Qed.
-
-(* Do the same thing as above
-   for state_list and ctrl_list (including the lemmas)*)
-Fixpoint state_list_equal (s1 : list State) (s2 : list State) :=
-  match s1, s2 with
-  | nil, nil => true
-  | s::y, s'::y' => andb (state_equal s s') (state_list_equal y y')
-  | _, _ => false
-  end. 
-
-Lemma state_list_equal_lemma:
-  forall s1 s2,
-  state_list_equal s1 s2 = true ->
-  s1 = s2.
-Proof.
-  intros s1.
-  induction s1 as [|s1' s1''].
-  - destruct s2; simpl; congruence.
-  - destruct s2 as [|s2' s2''].
-    + simpl. congruence.
-    + intros H. simpl in H.
-      rewrite andb_true_iff in H. destruct H as [H1 H2].
-      apply state_equal_lemma in H1. subst. f_equal.
-      apply IHs1''.
-      assumption.
-Qed.
-
-Fixpoint ctrl_list_equal (c1 : list Ctrl) (c2 : list Ctrl) :=
-  match c1, c2 with
-  | nil, nil => true
-  | c::y, c'::y' => andb (ctrl_equal c c') (ctrl_list_equal y y')
-  | _, _ => false
-  end.
-
-Lemma ctrl_equal_lemma :
-  forall c1 c2,
-  ctrl_equal c1 c2 = true ->
-  c1 = c2.
-Proof.
-  intros c1 c2 H.
-  destruct c1, c2; simpl in H; try congruence.
-  apply Pos.eqb_eq in H. subst. reflexivity.
-Qed.
-
-Lemma ctrl_list_equal_lemma:
-  forall c1 c2,
-  ctrl_list_equal c1 c2 = true ->
-  c1 = c2.
-Proof.
-  intros c1.
-  induction c1 as [|c1' c1''].
-  - destruct c2; simpl; congruence.
-  - destruct c2 as [|c2' c2''].
-    + simpl. congruence.
-    + intros H. simpl in H.
-      rewrite andb_true_iff in H. destruct H as [H1 H2].
-      apply ctrl_equal_lemma in H1. subst. f_equal.
-      apply IHc1''.
-      assumption.
-Qed.
+  Lemma varlike_list_equal_lemma :
+    forall v1 v2,
+    varlike_list_equal v1 v2 = true ->
+    v1 = v2.
+  Proof.
+    intros.
+    revert v2 H0.
+    induction v1 as [|v1' v1''].
+    - destruct v2.
+      + reflexivity.
+      + discriminate.
+    - destruct v2 as [|v2' v2''].
+      + intros. simpl in *. congruence.
+      + intros. simpl in *.
+        rewrite andb_true_iff in H0. destruct H0.
+        apply varlike_equal_lemma in H0.
+        apply IHv1'' in H1.
+        rewrite H0. rewrite <- H1. reflexivity.
+  Qed.
+End CrVarLikeEqual.
